rich_raven_lang/trnsl.v
@@ -774,12 +774,26 @@ Section MainTranslation.
 
         - destruct b0.
 
-          + setoid_rewrite trnsl_assertion_unfold. iIntros "[[Hstk Hu] Hcr]".
+          + 
+          (* setoid_rewrite trnsl_assertion_unfold. *)
+          iIntros (Φ). iModIntro.
+          iIntros "[Hstk Hcr] Hpost'".
 
-          iPoseProof ("IH'" with "[%] [Hstk Hu Hcr]") as "Hpost"; try iFrame; try done.
-          { unfold LExpr_holds. rewrite Hinterp_lexpr. done. }
+          setoid_rewrite trnsl_assertion_unfold.
+          iPoseProof ("IH'" with "[%] [Hstk Hcr]") as "Hpost"; try iFrame; try done.
+          { simpl. iDestruct "Hstk" as "[Hstk Htrnsl]". iFrame. iPureIntro. unfold LExpr_holds. rewrite Hinterp_lexpr. done. }
 
           iDestruct "Hpost" as ">[[Hstk Hu0] Hcr2]".
+
+          iApply (wp_skip (trnsl_assertion (LAnd (LStack stk2) q) stk_id mp) with "[Hstk Hu0]").
+          { setoid_rewrite trnsl_assertion_unfold. simpl. iFrame.  }
+
+          iNext. iIntros "Hpost1".
+          iApply "Hpost'".
+
+          setoid_rewrite trnsl_assertion_unfold.
+
+          iDestruct "Hpost1" as "[[Hstk Hu] Hcr]".
 
           assert (ι2 = ι2 `min` ι3 + (ι2 - ι2 `min` ι3)) as Hiota. { lia.  }
           apply (f_equal lc) in Hiota.
@@ -787,14 +801,29 @@ Section MainTranslation.
 
           iDestruct (lc_split (ι2 `min` ι3) (ι2 - (ι2 `min` ι3)) with "Hcr2") as "[Hcr2 Hcr2']".
 
-          iFrame. iModIntro. done.
+          iFrame.
           
-          + setoid_rewrite trnsl_assertion_unfold. iIntros "[[Hstk Hu] Hcr]".
+          + 
+          (* setoid_rewrite trnsl_assertion_unfold. *)
+          iIntros (Φ). iModIntro.
+          iIntros "[Hstk Hcr] Hpost'".
 
-          iPoseProof ("IH1'" with "[%] [Hstk Hu Hcr]") as "Hpost"; try iFrame; try done.
-          { unfold LExpr_holds. simpl.  rewrite Hinterp_lexpr. done. }
+
+          
+          (* iIntros "[[Hstk Hu] Hcr]". *)
+          setoid_rewrite trnsl_assertion_unfold.
+          iPoseProof ("IH1'" with "[%] [Hstk Hcr]") as "Hpost"; try iFrame; try done.
+          { simpl. iDestruct "Hstk" as "[Hstk Htrnsl]". iFrame. iPureIntro. unfold LExpr_holds. simpl. rewrite Hinterp_lexpr. done.  }
 
           iDestruct "Hpost" as ">[[Hstk Hu0] Hcr2]".
+
+          iApply (wp_skip (trnsl_assertion (LAnd (LStack stk2) q) stk_id mp) with "[Hstk Hu0]").
+          { setoid_rewrite trnsl_assertion_unfold. simpl. iFrame.  }
+
+          iNext. 
+          setoid_rewrite trnsl_assertion_unfold.
+          iIntros "[[Hstk Hu] Hcr]".
+          iApply "Hpost'".
 
           assert (ι3 = ι2 `min` ι3 + (ι3 - ι2 `min` ι3)) as Hiota. { lia.  }
           apply (f_equal lc) in Hiota.
@@ -802,7 +831,6 @@ Section MainTranslation.
 
           iDestruct (lc_split (ι2 `min` ι3) (ι3 - (ι2 `min` ι3)) with "Hcr2") as "[Hcr2 Hcr2']".
           iFrame.
-          done.
 
         - iIntros (Φ). iModIntro. setoid_rewrite trnsl_assertion_unfold. iIntros "[[Hstk Hu] Hcr] HΦ".
           destruct b0.
